updated q2

A1/Q2.dfy
@@ -6,6 +6,7 @@ reads a;
     forall j, k :: min <= j < k < max ==> a[j] <= a[k]
 }
 
+// Find the smaller one, a[left] or a[right]
 function min (a: array<int>, left: int, right: int): int
     requires a != null && a.Length > 0;
     requires 0 < left <= right < a.Length;
@@ -14,6 +15,7 @@ function min (a: array<int>, left: int, right: int): int
     if (a[left] > a[right]) then a[right] else a[left]
 }
 
+// Find the bigger one, a[right] or a[left]
 function max (a: array<int>, left: int, right: int): int
     requires a != null && a.Length > 0;
     requires 0 < left <= right < a.Length;
@@ -22,17 +24,42 @@ function max (a: array<int>, left: int, right: int): int
     if (a[left] > a[right]) then a[left] else a[right]
 }
 
+// Find minimum element in the array between left and right
+function findMin (a: array<int>, left: int, right: int): int
+    requires a != null && a.Length > 0;
+    requires 0 < left <= right < a.Length;
+    reads a;
+    decreases right - left;
+{
+    if (left == right) then a[left] else 
+        if (a[left] < a[right]) then findMin(a, left, right - 1) else findMin(a, left + 1, right)
+}
+
+// Find maximum element in the array between left and right
+function findMax (a: array<int>, left: int, right: int): int
+    requires a != null && a.Length > 0;
+    requires 0 < left <= right < a.Length;
+    reads a;
+    decreases right - left;
+{
+    if (left == right) then a[left] else 
+        if (a[left] < a[right]) then findMax(a, left + 1, right) else findMax(a, left, right - 1)
+}
+
 method stoogeSort(a: array <int>, left: int, right: int) 
+    decreases left;
+    decreases right;
     requires a != null;
     requires a.Length > 0;
     requires 1 <= left <= right <= a.Length - 1;
     modifies a;
     ensures sorted(a, left, right);
     ensures forall i :: (0 <= i < left || right < i < a.Length) ==> a[i] == old(a[i]);
-    ensures a[left] == min(a,left,right);
-    ensures a[right] == max(a,left,right);
-    ensures min(a, left, right) == old(min(a, left, right));
-    ensures max(a, left, right) == old(max(a, left, right));
+    ensures a[left] == findMin(a,left,right);
+    ensures a[right] == findMax(a,left,right);
+    ensures findMin(a, left, right) == old(findMin(a, left, right));
+    ensures findMax(a, left, right) == old(findMax(a, left, right));
+    decreases right - left;
 {
     if (a[left] > a[right]) {
         // swap a[left] and a[right]
@@ -90,29 +117,5 @@ method stoogeSort(a: array <int>, left: int, right: int)
 //             max := a[i]; 
 //         }
 //         i := i + 1;
-//     }
-// }
-
-// method min (a: array<int>, left: int, right: int) returns (min: int)
-//     requires a != null && a.Length > 0;
-//     requires left <= right <= a.Length;
-//     ensures a[left] <= a[right];
-// {
-//     if (a[left] > a[right]) {
-//         min := a[right];
-//     } else {
-//         min := a[left];
-//     }
-// }
-
-//  method max (a: array<int>, left: int, right: int) returns (max: int)
-//     requires a != null && a.Length > 0;
-//     requires left <= right <= a.Length;
-//     ensures a[left] <= a[right];
-// {
-//     if (a[left] > a[right]) {
-//         max := a[left];
-//     } else {
-//         max := a[right];
 //     }
 // }
